pulse/src/ocaml/plugin/generated/Pulse_Checker_Auto_IntroPure.ml
@@ -1,0 +1,179 @@
+open Prims
+let (is_pure : Pulse_Syntax_Base.term -> Prims.bool) =
+  fun p ->
+    match p with
+    | Pulse_Syntax_Base.Tm_Pure (Pulse_Syntax_Base.Tm_FStar (uu___, uu___1))
+        -> true
+    | uu___ -> false
+let (get_one_pure :
+  Pulse_Typing.env ->
+    Pulse_Syntax_Base.vprop Prims.list ->
+      (Pulse_Syntax_Base.vprop, Pulse_Syntax_Base.vprop Prims.list, unit)
+        FStar_Pervasives.dtuple3 FStar_Pervasives_Native.option)
+  = fun g -> fun l -> Prims.admit ()
+let (intro_pure_tm : Pulse_Syntax_Base.term -> Pulse_Syntax_Base.st_term) =
+  fun p ->
+    Pulse_Typing.wr
+      (Pulse_Syntax_Base.Tm_STApp
+         {
+           Pulse_Syntax_Base.head =
+             (Pulse_Syntax_Pure.tm_pureapp
+                (Pulse_Syntax_Pure.tm_fvar
+                   (Pulse_Syntax_Base.as_fv
+                      (Pulse_Reflection_Util.mk_steel_wrapper_lid
+                         "intro_pure"))) FStar_Pervasives_Native.None p);
+           Pulse_Syntax_Base.arg_qual = FStar_Pervasives_Native.None;
+           Pulse_Syntax_Base.arg =
+             (Pulse_Syntax_Base.Tm_FStar
+                ((FStar_Reflection_Builtins.pack_ln
+                    (FStar_Reflection_Data.Tv_Const
+                       FStar_Reflection_Data.C_Unit)), FStar_Range.range_0))
+         })
+let (intro_pure_comp : Pulse_Syntax_Base.term -> Pulse_Syntax_Base.comp) =
+  fun p ->
+    Pulse_Syntax_Base.C_STGhost
+      (Pulse_Syntax_Base.Tm_EmpInames,
+        {
+          Pulse_Syntax_Base.u = Pulse_Syntax_Pure.u_zero;
+          Pulse_Syntax_Base.res = Pulse_Typing.tm_unit;
+          Pulse_Syntax_Base.pre = Pulse_Syntax_Base.Tm_Emp;
+          Pulse_Syntax_Base.post = (Pulse_Syntax_Base.Tm_Pure p)
+        })
+let (intro_pure_typing :
+  Pulse_Typing.env ->
+    Pulse_Syntax_Base.term ->
+      unit -> unit -> (unit, unit, unit) Pulse_Typing.st_typing)
+  =
+  fun g ->
+    fun p ->
+      fun p_typing ->
+        fun p_valid ->
+          Pulse_Typing.T_STApp
+            (g,
+              (Pulse_Syntax_Pure.tm_pureapp
+                 (Pulse_Syntax_Pure.tm_fvar
+                    (Pulse_Syntax_Base.as_fv
+                       (Pulse_Reflection_Util.mk_steel_wrapper_lid
+                          "intro_pure"))) FStar_Pervasives_Native.None p), p,
+              FStar_Pervasives_Native.None, (intro_pure_comp p),
+              (Pulse_Syntax_Base.Tm_FStar
+                 ((FStar_Reflection_Builtins.pack_ln
+                     (FStar_Reflection_Data.Tv_Const
+                        FStar_Reflection_Data.C_Unit)), FStar_Range.range_0)),
+              (), ())
+let (intro_pure : Pulse_Checker_Auto_Util.intro_step_t) =
+  fun g ->
+    fun ctxt ->
+      fun pst ->
+        match get_one_pure g pst.Pulse_Checker_Auto_Util.unmatched_pre with
+        | FStar_Pervasives_Native.None ->
+            Obj.magic
+              (Obj.repr
+                 (FStar_Tactics_Effect.lift_div_tac
+                    (fun uu___ -> FStar_Pervasives_Native.None)))
+        | FStar_Pervasives_Native.Some (FStar_Pervasives.Mkdtuple3
+            (v, rest, veq)) ->
+            Obj.magic
+              (Obj.repr
+                 (FStar_Tactics_Effect.tac_bind
+                    (FStar_Range.mk_range "Pulse.Checker.Auto.IntroPure.fst"
+                       (Prims.of_int (71)) (Prims.of_int (45))
+                       (Prims.of_int (71)) (Prims.of_int (53)))
+                    (FStar_Range.mk_range "Pulse.Checker.Auto.IntroPure.fst"
+                       (Prims.of_int (71)) (Prims.of_int (56))
+                       (Prims.of_int (97)) (Prims.of_int (15)))
+                    (FStar_Tactics_Effect.lift_div_tac (fun uu___ -> ()))
+                    (fun uu___ ->
+                       (fun v_typing ->
+                          Obj.magic
+                            (FStar_Tactics_Effect.tac_bind
+                               (FStar_Range.mk_range
+                                  "Pulse.Checker.Auto.IntroPure.fst"
+                                  (Prims.of_int (72)) (Prims.of_int (20))
+                                  (Prims.of_int (72)) (Prims.of_int (21)))
+                               (FStar_Range.mk_range
+                                  "Pulse.Checker.Auto.IntroPure.fst"
+                                  (Prims.of_int (71)) (Prims.of_int (56))
+                                  (Prims.of_int (97)) (Prims.of_int (15)))
+                               (FStar_Tactics_Effect.lift_div_tac
+                                  (fun uu___ -> v))
+                               (fun uu___ ->
+                                  (fun uu___ ->
+                                     match uu___ with
+                                     | Pulse_Syntax_Base.Tm_Pure p ->
+                                         Obj.magic
+                                           (FStar_Tactics_Effect.tac_bind
+                                              (FStar_Range.mk_range
+                                                 "Pulse.Checker.Auto.IntroPure.fst"
+                                                 (Prims.of_int (74))
+                                                 (Prims.of_int (6))
+                                                 (Prims.of_int (74))
+                                                 (Prims.of_int (47)))
+                                              (FStar_Range.mk_range
+                                                 "Pulse.Checker.Auto.IntroPure.fst"
+                                                 (Prims.of_int (75))
+                                                 (Prims.of_int (4))
+                                                 (Prims.of_int (97))
+                                                 (Prims.of_int (15)))
+                                              (FStar_Tactics_Effect.lift_div_tac
+                                                 (fun uu___1 -> ()))
+                                              (fun uu___1 ->
+                                                 (fun p_typing ->
+                                                    Obj.magic
+                                                      (FStar_Tactics_Effect.tac_bind
+                                                         (FStar_Range.mk_range
+                                                            "Pulse.Checker.Auto.IntroPure.fst"
+                                                            (Prims.of_int (75))
+                                                            (Prims.of_int (10))
+                                                            (Prims.of_int (75))
+                                                            (Prims.of_int (58)))
+                                                         (FStar_Range.mk_range
+                                                            "Pulse.Checker.Auto.IntroPure.fst"
+                                                            (Prims.of_int (75))
+                                                            (Prims.of_int (4))
+                                                            (Prims.of_int (97))
+                                                            (Prims.of_int (15)))
+                                                         (Obj.magic
+                                                            (FStar_Tactics_Builtins.check_prop_validity
+                                                               (Pulse_Typing.elab_env
+                                                                  g)
+                                                               (Pulse_Elaborate_Pure.elab_term
+                                                                  p)))
+                                                         (fun uu___1 ->
+                                                            FStar_Tactics_Effect.lift_div_tac
+                                                              (fun uu___2 ->
+                                                                 match uu___1
+                                                                 with
+                                                                 | (FStar_Pervasives_Native.Some
+                                                                    e,
+                                                                    uu___3)
+                                                                    ->
+                                                                    FStar_Pervasives_Native.Some
+                                                                    {
+                                                                    Pulse_Checker_Auto_Util.v
+                                                                    = v;
+                                                                    Pulse_Checker_Auto_Util.unmatched'
+                                                                    = rest;
+                                                                    Pulse_Checker_Auto_Util.remaining'
+                                                                    =
+                                                                    (pst.Pulse_Checker_Auto_Util.remaining_ctxt);
+                                                                    Pulse_Checker_Auto_Util.t'
+                                                                    =
+                                                                    (intro_pure_tm
+                                                                    p);
+                                                                    Pulse_Checker_Auto_Util.c'
+                                                                    =
+                                                                    (intro_pure_comp
+                                                                    p);
+                                                                    Pulse_Checker_Auto_Util.t'_typing
+                                                                    =
+                                                                    (intro_pure_typing
+                                                                    g p () ());
+                                                                    Pulse_Checker_Auto_Util.unmatched_equiv
+                                                                    = ();
+                                                                    Pulse_Checker_Auto_Util.remaining_equiv
+                                                                    = ()
+                                                                    }
+                                                                 | uu___3 ->
+                                                                    FStar_Pervasives_Native.None))))
+                                                   uu___1))) uu___))) uu___)))
