pulse/src/ocaml/plugin/generated/Pulse_Checker_Auto_IntroRewrite.ml
@@ -1,0 +1,8 @@
+open Prims
+let (intro_rewrite : Pulse_Checker_Auto_Util.intro_step_t) =
+  fun g ->
+    fun ctxt ->
+      fun p ->
+        Obj.magic
+          (FStar_Tactics_Effect.lift_div_tac
+             (fun uu___ -> FStar_Pervasives_Native.None))
