pulse/lib/steel/pulse/Pulse.Checker.Auto.ElimPure.fsti
@@ -1,14 +1,13 @@
 module Pulse.Checker.Auto.ElimPure
-module RT = FStar.Reflection.Typing
-module R = FStar.Reflection
-module L = FStar.List.Tot
-module T = FStar.Tactics
-open FStar.List.Tot
+
 open Pulse.Syntax
-open Pulse.Checker.Pure
-open Pulse.Checker.Common
 open Pulse.Typing
-module Metatheory = Pulse.Typing.Metatheory
+
+open Pulse.Checker.Common
+open Pulse.Checker.Auto.Util
+
+module T = FStar.Tactics
+
 
 val elim_pure (#g:env) (#ctxt:term) (ctxt_typing:tot_typing g ctxt Tm_VProp)
    : T.Tac (g':env { env_extends g' g } &
