pulse/lib/steel/pulse/Pulse.Checker.Auto.IntroExists.fst
@@ -1,0 +1,20 @@
+module Pulse.Checker.Auto.IntroExists
+
+module RT = FStar.Reflection.Typing
+module R = FStar.Reflection
+module L = FStar.List.Tot
+module T = FStar.Tactics
+open FStar.List.Tot
+
+open Pulse.Syntax
+open Pulse.Checker.Pure
+open Pulse.Checker.Common
+open Pulse.Checker.VPropEquiv
+
+open Pulse.Typing
+
+module Metatheory = Pulse.Typing.Metatheory
+
+let intro_exists =
+  fun #g #ctxt p ->
+  None
