pulse/lib/steel/pulse/Pulse.Checker.Auto.IntroExists.fsti
@@ -1,0 +1,7 @@
+module Pulse.Checker.Auto.IntroExists
+
+open Pulse.Syntax
+open Pulse.Checker.Common
+open Pulse.Checker.Auto.Util
+
+val intro_exists : intro_step_t
