pulse/lib/steel/pulse/Pulse.Checker.Common.fsti
@@ -111,16 +111,10 @@ let comp_post_matches_hint (c:comp_st) (post_hint:option post_hint_t) =
     comp_u c == post_hint.u /\
     comp_post c == post_hint.post
 
-let checker_result_t (g:env) (ctxt:term) (post_hint:option post_hint_t) =
+type checker_result_t (g:env) (ctxt:term) (post_hint:option post_hint_t) =
     t:st_term &
     c:comp{stateful_comp c ==> (comp_pre c == ctxt /\ comp_post_matches_hint c post_hint) } &
     st_typing g t c
-
-let continuation_elaborator (g:env) (ctxt:term)
-                            (g':env) (ctxt':term) =
-    post_hint:post_hint_opt g ->
-    checker_result_t g' ctxt' post_hint ->
-    T.Tac (checker_result_t g ctxt post_hint)
 
 type check_t =
   g:env ->
